README.md
@@ -1,16 +1,22 @@
-The Logic of Delay
-==================
-The aim of this project is to formalize propositional logic with the later
-modality. This modality is used by the Iris framework to prove properties of
-recursive programs [1]. This technique is also called guarded recursion [2]. We
-introduce a new axiom to prove completeness. This axiom states the following:
-For all formulas P and Q, either P implies Q, or later Q implies P.
+A Complete Proof System for the Later Modality
+==============================================
 
-To build the files in this repository, use:
+[![DOI](https://zenodo.org/badge/DOI/10.5281/zenodo.6347180.svg)](https://doi.org/10.5281/zenodo.6347180)
+
+The aim of this project is to formalize propositional logic with the *later*
+modality. This modality is used by the *Iris* framework ([1]) as a technique to
+prove properties of recursive programs ([2]), which is also called guarded
+recursion ([3]). We introduce a new axiom to prove completeness:
+
+*For all formulas P and Q, either P implies Q, or later Q implies P.*
+
+Verify
+------
 ```
 coq_makefile -f _CoqProject -o CoqMakefile
 make -f CoqMakefile
 ```
 
-[1]: https://iris-project.org/tutorial-pdfs/lecture7-later.pdf
-[2]: https://ncatlab.org/nlab/show/guarded+recursion
+[1]: https://iris-project.org/
+[2]: https://iris-project.org/tutorial-pdfs/lecture7-later.pdf
+[3]: https://ncatlab.org/nlab/show/guarded+recursion
